Finish some more subgoals of the recovery refinement proof.

src/Examples/MailServer/MailRefinement.v
@@ -43,6 +43,8 @@ Definition init_base `{@GoModelWf gm} (s: GoLayer.Go.State) :=
       (uid < 100 -> s.(fs).(dirents) !! (UserDir uid) = Some ∅) ∧
       (uid >= 100 -> s.(fs).(dirents) !! (UserDir uid) = None)) ∧
   s.(fs).(FS.dirents) !! SpoolDir = Some ∅ ∧
+  (∀ d, is_Some (s.(fs).(FS.dirents) !! d) →
+        d = SpoolDir ∨ (∃ uid, d = UserDir uid)) ∧
   dom (gset string) s.(fs).(FS.dirents) =
   dom (gset string) s.(fs).(FS.dirlocks) ∧
   (∀ dir l, s.(fs).(FS.dirlocks) !! dir = Some l → fst l = Unlocked) ∧
@@ -58,6 +60,59 @@ Definition myΣ {gm} {Hgwf: GoModelWf gm} : gFunctors :=
 Existing Instance subG_goosePreG.
 Existing Instance subG_cfgPreG.
 
+Lemma init_dirs {gm} {Hgwf: GoModelWf gm} σ1a σ1c:
+  init_absr σ1a σ1c →
+  dom (gset string) σ1c.(fs).(dirents) =
+                  (set_map UserDir (dom (gset uint64) σ1a.(messages)) ∪ {[SpoolDir]}).
+Proof.
+  intros (Hinita&Hinitc).
+  destruct Hinita as (Hheap&?&Hrange).
+  destruct Hinitc as (Hheap'&Hrange'&Hspool&Hdirs&Hlocks1&Hlocks2).
+  assert (dom (gset string) σ1c.(fs).(dirents) =
+          (set_map UserDir (dom (gset uint64) σ1a.(messages)) ∪ {[SpoolDir]})) as ->; auto.
+  rewrite -leibniz_equiv_iff => d.
+  split.
+  * intros Hin. apply elem_of_dom in Hin. edestruct (Hdirs d) as [|(uid&Heq)]; eauto.
+    ** subst. set_solver+.
+    ** rewrite Heq.
+       destruct (lt_dec uid 100); last first.
+       { exfalso. destruct (Hrange' uid) as (?&Hnone). subst.
+         rewrite Hnone in Hin; try lia. eapply is_Some_None; eauto.
+       }
+       apply elem_of_union_l. apply elem_of_map.
+       exists uid; split; eauto.
+       apply elem_of_dom. destruct (Hrange uid) as (Hsome&?).
+       rewrite Hsome; auto. eauto.
+  * intros [Huser|Hisspool]%elem_of_union.
+    ** apply elem_of_dom. apply elem_of_map in Huser as (uid&Heq&Hin).
+       apply elem_of_dom in Hin.
+       subst.
+       destruct (lt_dec uid 100); last first.
+       { exfalso. destruct (Hrange uid) as (?&Hnone).
+         rewrite Hnone in Hin; try lia. eapply is_Some_None; eauto.
+       }
+       destruct (Hrange' uid) as (Hsome&?).
+       rewrite Hsome; eauto.
+    ** apply elem_of_singleton in Hisspool. subst.
+       eapply elem_of_dom; eauto.
+Qed.
+
+Lemma init_base_dirs_empty `{@GoModelWf gm} σ dir x:
+  init_base σ →
+  σ.(fs).(dirents) !! dir = Some x →
+  x = ∅.
+Proof.
+  intros (_&Hrange&Hspool&Hdom&_).
+  intros Hsome. destruct (Hdom dir) as [|(uid&?)]; eauto.
+  * subst. congruence.
+  * destruct (lt_dec uid 100); last first.
+    { exfalso. destruct (Hrange uid) as (?&Hnone). subst.
+      rewrite Hnone in Hsome; try lia. congruence.
+    }
+    destruct (Hrange uid) as (Hsome'&?).
+    subst. rewrite Hsome' in Hsome; try lia. congruence.
+Qed.
+
 Lemma mail_crash_refinement_seq {gm} {Hgmwf: @GoModelWf gm} {T} σ1c σ1a esa esc:
   init_absr σ1a σ1c →
   wf_client_seq esa →
@@ -72,11 +127,8 @@ Proof.
       (es := esa)
       (T := T)
       (exec_inv := fun H1 H2 => (∃ hGTmp, @ExecInv gm Hgmwf myΣ H2 H1 _ _ hGTmp)%I)
-      (exec_inner := fun H1 H2 => True%I)
-      (crash_inner := fun H1 H2 => True%I)
-      (*
-      (crash_inner := fun H1 H2 => (@CrashInner myΣ H2 H1)%I)
-       *)
+      (exec_inner := fun H1 H2 => (∃ hGTmp, @ExecInner gm Hgmwf myΣ H2 H1 _ _ hGTmp)%I)
+      (crash_inner := fun H1 H2 => @CrashInner gm Hgmwf myΣ H2 H1 _ _)
       (crash_param := fun H1 H2 => unit)
       (crash_inv := fun H1 H2 _ => @CrashInv _ _ myΣ H2 H1 _ _)
       (crash_starter := fun H1 H2 _ => @CrashStarter _ _ myΣ H2)
@@ -129,7 +181,7 @@ Proof.
          this point, it is totally irrelevant *)
       wp_ret. wp_ret. iNext.
       iInv "Hinv" as "H" "_".
-      iDestruct "H" as (σ) "(>Hstate&Hmsgs&>Hheap&>Htmp)".
+      iDestruct "H" as (σ) "(>Hstate&>Hmsgs&>Hheap&>Htmp)".
       iApply (fupd_mask_weaken _ _).
       { solve_ndisj. }
       iExists _, _.
@@ -137,8 +189,19 @@ Proof.
       { iPureIntro. do 2 eexists; split; econstructor. }
       iClear "Hsource".
       iIntros (???) "(#Hsource&Hstate)".
-      (* todo: prove execinner for new run *)
-      admit.
+      iDestruct "Htmp" as (tmps_map) "(Hdir&Hpaths)".
+      iDestruct (mapsto_agree with "[$] [$]") as %Heq_dom.
+      rewrite <-Heq_dom.
+      iDestruct (read_split_join with "[Htmps Hdir]") as "Hdir".
+      { iFrame. replace 1%Z with (S O : Z) by auto. iFrame. }
+      iMod (gen_heap_init tmps_map) as (hGTmp) "Htmp".
+      iExists hGTmp, Γ, γ, _.
+      iFrame.
+      iSplitL "".
+      { eauto. }
+      iSplitL "Hmsgs".
+      { by iApply MsgsInv_crash_set_false. }
+      iExists _. by iFrame.
     - wp_bind.
       destruct (nth_error ltmps i) as [curr_name|] eqn:Heq_curr_name; last first.
       { exfalso. eapply nth_error_Some; eauto.  inversion Hlen; try congruence; try lia. }
@@ -159,11 +222,13 @@ Proof.
       iDestruct (big_sepM_delete with "Hpaths") as "(Hcurr&Hpaths)"; eauto.
       iApply (wp_delete with "[$]").
       iIntros "!> (Hdir&Hdirlock)".
-      iExists _. iFrame.
       iDestruct (read_split_join _ 0 with "Hdir") as "(Hdir&Htmps)".
-      iSplitL "Hdir Hpaths".
-      { iModIntro. iNext. iExists _. iFrame.
-        rewrite dom_delete_L. rewrite Heq_dom. iFrame. }
+      iSplitL "Hstate Hmsgs Hheap Hpaths Hdir".
+      {
+        iExists _. iFrame.
+        iModIntro. iNext. iExists _. iFrame.
+        rewrite dom_delete_L. rewrite Heq_dom. iFrame.
+      }
       wp_ret. iModIntro. iNext.
       iApply ("IH" with "[] [$] [$] [$] [Htmps]").
       { iPureIntro. inversion Hlen; try congruence; try lia. }
@@ -171,4 +236,147 @@ Proof.
       (* todo: prove list_to_set (take (i+1 ltmps) gives you union of take i ltmps with curr *)
       admit.
   }
+  { rewrite /init_absr/initP/init_base. intuition. }
+  { clear. iIntros (σ1a σ1c Hinit).
+    iIntros (??) "(Hdirs&Hroot&Hdirlocks&Hsrc&Hstate&Hglobal)".
+    pose proof (init_dirs _ _ Hinit) as Hdirs.
+    destruct Hinit as (Hinita&Hinitc).
+    iMod (gen_heap_init (∅: gmap string Inode)) as (hGTmp) "Htmp".
+    iExists hGTmp.
+    iMod (ghost_var_alloc (A := @ghost_init_statusC gm Hgmwf) Uninit) as "H".
+    iDestruct "H" as (γ) "(Hauth&Hfrag)".
+    iMod (ghost_var_bulk_alloc (A := contentsC) (σ1a.(messages)) (λ _ _, ∅)) as "H".
+    iDestruct "H" as (Γ HΓdom) "HΓ".
+    iAssert ([∗ map] k↦_ ∈ σ1a.(messages), ∃ γ0 : gname, ⌜Γ !! k = Some γ0⌝)%I
+            with "[HΓ]" as "#HΓ'".
+    { iApply big_sepM_mono; last eauto. iIntros (???) "H". iDestruct "H" as (?) "(?&?)"; eauto. }
+    iExists Γ, γ, σ1a. iFrame.
+    assert (SpoolDir ∈ dom (gset string) σ1c.(fs).(dirents)).
+    { rewrite /init_base in Hinitc. intuition.
+      apply elem_of_dom. eexists; eauto.
+    }
+    iSplitL "".
+    { iPureIntro. destruct Hinita as (?&->&?); auto. }
+    iDestruct (big_opS_delete with "Hdirlocks") as "(Hlock&Hdirlocks)"; eauto.
+    iDestruct (big_opM_delete with "Hdirs") as "(Hspool&Hdirs)".
+    { rewrite /init_base in Hinitc. intuition. eauto. }
+    iSplitR "Htmp Hlock Hspool".
+    { rewrite /MsgsInv. iExists [].
+      rewrite /initP in Hinita.
+      destruct Hinita as (Hheap&Hopen&Hrange).
+      rewrite Hopen.
+      iFrame.
+      iSplitL "Hroot".
+      { iModIntro. rewrite /RootDirInv. iSplitR ""; last first.
+        - iPureIntro.  rewrite /userRange_ok => uid.
+          destruct (Hrange uid). split; intros.
+          * apply elem_of_dom; eexists; eauto.
+          * apply not_elem_of_dom; eauto.
+        - rewrite /init_base in Hinitc.
+          rewrite Hdirs. eauto.
+      }
+      iSplitR "Hdirs Hdirlocks"; last first.
+      {rewrite -dom_delete_L.
+        iDestruct (big_sepM_dom with "Hdirlocks") as "Hdirlocks".
+        iAssert ([∗ map] uid↦lm ∈ σ1a.(messages), MsgInv Γ [] uid (MUnlocked, ∅) false)%I
+                 with "[Hdirs Hdirlocks]" as "H"; last first.
+        { iModIntro. iApply big_sepM_mono; last eauto. admit. }
+        iAssert ([∗ map] k↦y ∈ base.delete SpoolDir σ1c.(fs).(dirents), k ↦ ∅)%I
+          with "[Hdirs]" as "Hdirs".
+        { iApply big_sepM_mono; last eauto.
+          iIntros (dir x Hin) "Hk".
+          cut (x = ∅).
+          { intros ->. by rewrite dom_empty_L. }
+          apply lookup_delete_Some in Hin as (Hneq&Hlookup).
+          destruct (Hinitc) as (?&Hrange'&_).
+          eapply init_base_dirs_empty; eauto.
+        }
+        assert (Hdirs_delete : dom (gset string) (map_delete SpoolDir (σ1c.(fs).(dirents))) =
+                               set_map UserDir (dom (gset uint64) σ1a.(messages))).
+        { admit. }
+        move: Hdirs_delete.
+        rewrite /base.delete.
+        generalize ((map_delete SpoolDir σ1c.(fs).(dirents))) => dirs.
+        generalize (σ1a.(messages)) => msgs.
+        clear Hrange Hdirs Hheap H => Hdom.
+        iInduction msgs as [|k i m] "IH" using map_ind forall (dirs Hdom).
+        { by iApply big_sepM_empty. }
+        rewrite big_sepM_insert //.
+        rewrite big_sepM_insert //.
+        assert (∃ v, dirs !! (UserDir k) = Some v) as (v&Hin).
+        { admit. }
+        iDestruct (big_sepM_delete with "Hdirlocks") as "(Hlock&Hdirlocks)"; first eauto.
+        iDestruct (big_sepM_delete with "Hdirs") as "(Hdir&Hdirs)"; first eauto.
+        iDestruct "HΓ'" as "(Hghost&HΓ')".
+        iSplitL "Hlock Hdir Hghost".
+        { iDestruct "Hghost" as (γuid) "H".
+          iExists (zeroValue _), γuid. iFrame.
+          simpl. rewrite dom_empty_L. iFrame.
+          iSplitL ""; auto.
+        }
+        iApply ("IH" with "[] [$] [$] [$]").
+        iPureIntro. rewrite dom_insert_L in Hdom.
+        rewrite dom_delete_L.
+        rewrite Hdom.
+        admit.
+      }
+      iExists _. iFrame. iFrame.
+      iSplitL ""; auto.
+      iModIntro. iApply big_sepM_mono; last iApply "HΓ".
+      iIntros (???) "H".
+      iDestruct "H" as (γuid) "(?&?&?)".
+      iExists _. iFrame. iExists _, _. iFrame.
+    }
+    { iSplitL "".
+      - rewrite /HeapInv. rewrite /initP in Hinita. destruct Hinita as (->&?).
+        simpl. iModIntro. by iApply big_sepDM_empty.
+      - iExists ∅. iFrame. by iApply big_sepM_empty.
+    }
+  }
+  {
+    iIntros (??) "H".
+    iDestruct "H" as (hGtmp) "Hrest".
+    iDestruct "Hrest" as (Γ γ) "(#Hsource&#Hinv)".
+    iInv "Hinv" as "H" "_".
+    iDestruct "H" as (σ) "(>Hstate&Hmsgs&>Hheap&>Htmp)".
+    iApply (fupd_mask_weaken _ _).
+    { solve_ndisj. }
+    iDestruct "Hmsgs" as (?) "(_&>Hroot&Hinit&Hmsgs)".
+    iIntros (?????) "(Hroot'&Hglobal)".
+    iDestruct "Hroot'" as (S) "(Hroot'&Hdirlocks)".
+    iDestruct "Hroot" as "(Hroot&%)".
+    iDestruct (ghost_var_agree2 (A := discreteC (gset string))_ with "Hroot Hroot'") as %Heq_dom.
+    iModIntro.
+    iExists _, _, _. iFrame.
+    iDestruct "Htmp" as (tmps_map) "(Hspool&_&Htmps&Hpaths)".
+    replace 0%Z with (O : Z) by auto.
+    iDestruct (read_split_join with "Hspool") as "(Hspool1&Hspool2)".
+    rewrite <-Heq_dom.
+    (*
+    iSplitR "Hspool2 Hspoollock"; last first.
+    { iExists _. iFrame.
+      replace 0%Z with (O : Z) by auto.
+      iFrame.
+     *)
+    admit.
+  }
+  { admit. }
+  { iIntros (??) "(H1&H2)". iDestruct "H1" as (Hinv) "(H&Hstarter)".
+    iDestruct "H" as (???) "(?&?&?)".
+    iExists _. iFrame.
+    iExists _, _. iFrame.
+    iMod (@inv_alloc myΣ (go_invG) execN _ _ with "[-]"); last eauto.
+    iNext. iExists _. iFrame.
+  }
+  { iIntros (??) "(H1&H2)". iDestruct "H1" as (Hinv hGTmp ??? Hclosed) "(Hstate&Hmsgs&Heap&Htmps)".
+    iExists hGTmp.
+    iExists _, _. iFrame.
+    iMod (@inv_alloc myΣ (go_invG) execN _ _ with "[-]"); last eauto.
+    iNext. iExists _. iFrame "Hstate Heap Htmps".
+    rewrite /MsgsInv.
+    iDestruct "Hmsgs" as (?) "(Hglobal&Hroot&Hinit&Hmsgs)".
+    iExists _. iFrame "Hglobal Hroot Hinit".
+    rewrite Hclosed. eauto.
+  }
+  { admit. }
 Abort.
